@prefix mat-lbl:        <https://w3id.org/i40/mat-lbl#> .
@prefix cc:      <http://creativecommons.org/ns#> .
@prefix dc:      <http://purl.org/dc/terms/> .
@prefix dc11:    <http://purl.org/dc/elements/1.1/> .
@prefix dct:     <http://purl.org/dc/terms/> .
@prefix deo:     <http://purl.org/spar/deo/> .
@prefix foaf:    <http://xmlns.com/foaf/0.1/> .
@prefix muto:    <http://purl.org/muto/core#> .
@prefix owl:     <http://www.w3.org/2002/07/owl#> .
@prefix rami:    <https://w3id.org/i40/rami#> .
@prefix rdf:     <http://www.w3.org/1999/02/22-rdf-syntax-ns#> .
@prefix rdfs:    <http://www.w3.org/2000/01/rdf-schema#> .
@prefix schema:  <http://schema.org/> .
@prefix skos:    <http://www.w3.org/2004/02/skos/core#> .
@prefix vann:    <http://purl.org/vocab/vann/> .
@prefix voaf:    <http://purl.org/vocommons/voaf#> .
@prefix xml:     <http://www.w3.org/XML/1998/namespace> .
@prefix xsd:     <http://www.w3.org/2001/XMLSchema#> .
@prefix geo:     <http://www.geonames.org/ontology#> .
@prefix dbo:     <http://dbpedia.org/ontology#> .
@prefix dbr:     <http://dbpedia.org/resource#> .
@prefix dul:     <http://www.ontologydesignpatterns.org/ont/dul/DUL.owl#> .
@prefix conti:     <http://www.continental.com/vocab/products#> .

mat-lbl: rdf:type owl:Ontology ;
      dc11:description "A vocabulary to describe the Requirements on Marking of Goods and Accompanying Information for Purchased Production Parts" ;
      dc11:title "MAT-Label Vocabulary"@en ;
      dc:created "2017-08-23"^^xsd:date ;
      dct:creator <https://orcid.org/0000-0002-1019-3606> , 
                  <http://sda.cs.uni-bonn.de/people/irlan-grangel-gonzalez/> , 
                  <http://sda.cs.uni-bonn.de/people/niklas-petersen/> ,
                  <http://sda.cs.uni-bonn.de/people/lavdim-halilaj/> ;
      dc:publisher <http://de.dbpedia.org/resource/Fraunhofer-Gesellschaft> ;
      vann:preferredNamespacePrefix "mat-lbl" ;
      vann:preferredNamespaceUri "https://w3id.org/i40/mat-lbl#" ;
      owl:versionInfo "0.1" ;
.

<https://orcid.org/0000-0002-1019-3606>
    rdf:type schema:Person ;
    rdfs:label "Anna Kasprzik" ;
    schema:affiliation <http://dbpedia.org/resource/German_National_Library_of_Science_and_Technology> ;
.

<http://sda.cs.uni-bonn.de/people/irlan-grangel-gonzalez/>
    rdf:type schema:Person ;
    rdfs:label "Irlán Grangel-González" ;
    schema:affiliation <http://dbpedia.org/resource/University_of_Bonn> ;
.

<http://sda.cs.uni-bonn.de/people/niklas-petersen/>
    rdf:type schema:Person ;
    rdfs:label "Niklas Petersen" ;
    schema:affiliation <http://dbpedia.org/resource/University_of_Bonn> ;
.

<http://sda.cs.uni-bonn.de/people/lavdim-halilaj/>
    rdf:type schema:Person ;
    rdfs:label "Lavdim Halilaj" ;
    schema:affiliation <http://dbpedia.org/resource/University_of_Bonn> ;
.

################ General

mat-lbl:PartPackaging
      rdf:type owl:Class ;
      rdfs:label "PartPackaging"@en ;
      rdfs:comment "The smallest package does not contain any additional sub-packaging usually."@en ;
.

mat-lbl:MatLabel
      rdf:type owl:Class ;
      rdfs:label "MATLabel"@en ;
      rdfs:comment "A unique material label on the smallest package unit containing a clearly defined set of traceability information in human- and in machine-readable form."@en ;
.

mat-lbl:hasMatLabel
      rdf:type owl:ObjectProperty ;
      rdfs:label "hasMATLabel"@en ;
      rdfs:comment "The set of data fields assigned to a part package."@en ;
      rdfs:domain mat-lbl:PartPackaging ;
      rdfs:range mat-lbl:PartPackaging ;
.

mat-lbl:DataField
      rdf:type owl:Class ;
      rdfs:label "DataField"@en ;
      rdfs:comment "The Data Matrix Code on the MAT-Label has to contain all data fields including its data identifier in the order represented by the column number."@en ;
.

mat-lbl:hasDataField
      rdf:type owl:ObjectProperty ;
      rdfs:label "hasDataField"@en ;
      rdfs:comment "A MAT-label comprises a set of mandatory data fields."@en ;
      rdfs:domain mat-lbl:PartPackaging ;
      rdfs:range mat-lbl:DataField ;
.

mat-lbl:Manufacturer
      rdf:type owl:Class;
      rdfs:subClassOf dbo:Company ;
      rdfs:label "Manufacturer"@en;
      rdfs:comment "A company that produces goods in large numbers."@en;
.

mat-lbl:hasManufacturer
      rdf:type owl:ObjectProperty ;
      rdfs:label "hasManufacturer"@en ;
      rdfs:comment "A company that produces goods in large numbers."@en ;
      rdfs:domain mat-lbl:PartPackaging ;
      rdfs:range mat-lbl:Manufacturer ;
.

mat-lbl:Supplier
      rdf:type owl:Class;
      rdfs:subClassOf dbo:Company ;
      rdfs:label "Supplier"@en;
      rdfs:comment "A company that delivers parts to customers."@en;
.

mat-lbl:hasSupplier
      rdf:type owl:ObjectProperty ;
      rdfs:label "hasSupplier"@en ;
      rdfs:comment "A company that delivers parts to customers."@en ;
      rdfs:domain mat-lbl:PartPackaging ;
      rdfs:range mat-lbl:Supplier ;
.

mat-lbl:Customer
      rdf:type owl:Class;
      rdfs:subClassOf dbo:Company ;
      rdfs:label "Customer"@en;
      rdfs:comment "An industrial plant that orders and receives goods."@en;
.

mat-lbl:hasCustomer
      rdf:type owl:ObjectProperty ;
      rdfs:label "hasCustomer"@en ;
      rdfs:comment "An industrial plant that orders and receives goods."@en ;
      rdfs:domain mat-lbl:PartPackaging ;
      rdfs:range mat-lbl:Customer ;
.

################ Data fields

mat-lbl:hasDataContent
      rdf:type owl:DatatypeProperty ;
      rdfs:label "hasDataContent"@en ;
      rdfs:comment "If mutual agreed, blanks are only permissible in the data fields, if they are part of the information content or if they were provided to the supplier as stated in the order."@en ;
      rdfs:domain mat-lbl:DataField ;
      rdfs:range xsd:string ; 
.

mat-lbl:DataID rdf:type rdfs:Datatype ;
      rdfs:comment "The content of each data field is described by a data identifier. Within each data field, the data identifier precedes the data." ;
      owl:equivalentClass [rdf:type rdfs:Datatype ; owl:onDatatype xsd:string ;
			   owl:withRestrictions ([xsd:pattern "([1-9]([0-9])?)?[A-Z]"])]
.

#mat-lbl:hasDataID
#      rdf:type owl:DatatypeProperty ;
#      rdfs:label "hasDataID"@en ;
#      rdfs:comment "The content of each data field is described by a data identifier. Within each data field, the data identifier precedes the data." ;
#      rdfs:domain mat-lbl:DataField ;
#      rdfs:range mat-lbl:DataID ; 
#.

mat-lbl:labelVersion
      a owl:DatatypeProperty ;
      rdfs:domain mat-lbl:PartPackaging;
      rdfs:range xsd:string ; 
      rdfs:label "LabelVersion"@en ;
      rdfs:comment "The revision level is a fixed entry and serves the recognition of the label or its version"@en ;
      skos:notation "12S"^^mat-lbl:DataID ; 
#      mat-lbl:hasDataID "12S"^^mat-lbl:DataID ;
.

mat-lbl:customerPartNumber
      a owl:DatatypeProperty ;
      rdfs:domain mat-lbl:PartPackaging;
      rdfs:range xsd:string ; 
      rdfs:label "CustomerPartNumber"@en ;
      rdfs:comment "Part number of the customer."@en ;
      skos:notation "P"^^mat-lbl:DataID ; 
.

mat-lbl:manufacturerPartNumber 
      a owl:DatatypeProperty ;
      rdfs:domain mat-lbl:PartPackaging;
      rdfs:range xsd:string ; 
      rdfs:label "ManufacturerPartNumber"@en ;
      rdfs:comment "Internal manufacturer part number."@en ;
      skos:example "SL105C103MAA-S" ;
      skos:notation "1P"^^mat-lbl:DataID ; 
.

mat-lbl:orderingCode 
      a owl:DatatypeProperty ;
      rdfs:domain mat-lbl:PartPackaging;
      rdfs:range xsd:string ; 
      rdfs:label "OrderingCode"@en ;
      rdfs:comment "Code for the part which non-ambigously can be used for ordering it. Compared to the Manufacturer Part number, the Ordering Code may obtain more information, e.g. Software Version in case of Microcontrollers or package form."@en ;
      skos:notation "31P"^^mat-lbl:DataID ; 
.

# PartDescription is no DataField and is not contained in the Data Matrix Code! However, it is contained in the printed label.
mat-lbl:partDescription 
      a owl:DatatypeProperty ;
      rdfs:domain mat-lbl:PartPackaging;
      rdfs:range xsd:string ; 
      rdfs:subClassOf mat-lbl:PrintedEntry ;
      rdfs:label "PartDescription"@en ;
      rdfs:comment "Clear-text description of the part (or part name), so that persons who are not familiar with the manufacturer's naming convention can understand what kind of component this is."@en ;
.

mat-lbl:manufacturerNumber 
      a owl:DatatypeProperty ;
      rdfs:domain mat-lbl:PartPackaging;
      rdfs:range xsd:string ; 
      rdfs:label "ManufacturerNumber"@en ;
      rdfs:comment "Explicit identification for the manufacturer, e.g. DUNS-Nr. or mutual agreed manufacturer number."@en ;
      skos:notation "12V"^^mat-lbl:DataID ; 
.

mat-lbl:manufacturerLocation 
      a owl:DatatypeProperty ;
      rdfs:domain mat-lbl:PartPackaging;
      rdfs:range xsd:string ; 
      rdfs:label "ManufacturerLocation"@en ;
      rdfs:comment "Naming of the manufacturing location / locations."@en ;
      skos:example "DEU-BERLIN - In case of only one location in town; DEU-BERLIN1, DEU-BERLIN2  - In case of two location in town" @en;
      skos:notation "10V"^^mat-lbl:DataID ; 
.

mat-lbl:revisionLevel 
      a owl:DatatypeProperty ;
      rdfs:domain mat-lbl:PartPackaging;
      rdfs:range xsd:string ; 
      rdfs:label "RevisionLevel"@en ;
      rdfs:comment "Revision status of the part."@en ;
      skos:notation "2P"^^mat-lbl:DataID ; 
.

mat-lbl:additionalPartInformation 
      a owl:DatatypeProperty ;
      rdfs:domain mat-lbl:PartPackaging;
      rdfs:range xsd:string ; 
      rdfs:label "AdditionalPartNumber"@en ;
      rdfs:comment "Used differently for each plan, flexible filled, e.g. brightness of the LEDs."@en ;
      skos:notation "20P"^^mat-lbl:DataID ; 
.

mat-lbl:manufacturingDate 
      a owl:DatatypeProperty ;
      rdfs:domain mat-lbl:PartPackaging;
      rdfs:range xsd:string ; 
      rdfs:label "ManufacturingDate"@en ;
      rdfs:comment "Date of manufacturing is related to the last manufacturing process."@en ;
      skos:notation "6D"^^mat-lbl:DataID ; 
.

mat-lbl:expirationDate 
      a owl:DatatypeProperty ;
      rdfs:domain mat-lbl:PartPackaging;
      rdfs:range xsd:string ; 
      rdfs:label "ExpirationDate"@en ;
      rdfs:comment "The Expiration Date of the part (defined by the manufacturer, depending on the production date)."@en ;
      skos:notation "14D"^^mat-lbl:DataID ; 
.

mat-lbl:rohs 
      a owl:DatatypeProperty ;
      rdfs:domain mat-lbl:PartPackaging;
      rdfs:range xsd:string ; 
      rdfs:label "RoHS"@en ;
      rdfs:comment "Indicator for RoHS (restriction of the use of certain hazardous substances in electrical and electronic equipment) compliance. N: no RoHS, Y: RoHS, 0: not acceptable."@en ;
      skos:notation "30P"^^mat-lbl:DataID ; 
.

mat-lbl:msLevel 
      a owl:DatatypeProperty ;
      rdfs:domain mat-lbl:PartPackaging;
      rdfs:range xsd:string ; 
      rdfs:label "MSlevel"@en ;
      rdfs:comment "Moisture Sensivity Level according to IPC/JEDEC J-STD-020."@en ;
      skos:notation "Z"^^mat-lbl:DataID ; 
.

mat-lbl:purchaseOrderNumber
      a owl:DatatypeProperty ;
      rdfs:domain mat-lbl:PartPackaging;
      rdfs:range xsd:string ; 
      rdfs:label "PurchaseOrderNumber"@en ;
      rdfs:comment "Order number assigned by customer to identify a purchasing transaction."@en ;
      skos:notation "K"^^mat-lbl:DataID ; 
.

mat-lbl:shippingNoteNumber 
      a owl:DatatypeProperty ;
      rdfs:domain mat-lbl:PartPackaging;
      rdfs:range xsd:string ; 
      rdfs:label "ShippingNoteNumber"@en ;
      rdfs:comment "Shipping Note Number of the shipping note and MAT-Label must be the same."@en ;
      skos:notation "16K"^^mat-lbl:DataID ; 
.

# SupplierName is no DataField and is not contained in the Data Matrix Code! However, it is contained in the printed label.
mat-lbl:supplierName 
      a owl:DatatypeProperty ;
      rdfs:domain mat-lbl:PartPackaging;
      rdfs:range xsd:string ; 
      rdfs:label "SupplierName"@en ;
      rdfs:comment "Name of the Supplier."@en ;
.

mat-lbl:supplierId 
      a owl:DatatypeProperty ;
      rdfs:domain mat-lbl:PartPackaging;
      rdfs:range xsd:string ; 
      rdfs:label "SupplierID"@en ;
      rdfs:comment "The vendor number (of the customer) for the supplier. It has to be taken over from the order.."@en ;
      skos:notation "V"^^mat-lbl:DataID ; 
.

mat-lbl:packageId 
      a owl:DatatypeProperty ;
      rdfs:domain mat-lbl:PartPackaging;
      rdfs:range xsd:string ; 
      rdfs:label "PackageID"@en ;
      rdfs:comment "The explicit, unique number per single package. It has to be unique per supplier-id (vendor number) and package. It is always related to the smallest package unit. If possible, chronologically related to the production process (e.g. reel-ID)."@en ;
      skos:notation "3S"^^mat-lbl:DataID ; 
.

mat-lbl:quantity 
      a owl:DatatypeProperty ;
      rdfs:domain mat-lbl:PartPackaging;
      rdfs:range xsd:double ; 
      rdfs:label "Quantity"@en ;
      rdfs:comment "Quantity of the smallest package unit"@en ;
      skos:notation "Q"^^mat-lbl:DataID ; 
.

mat-lbl:batchCounter 
      a owl:DatatypeProperty ;
      rdfs:domain mat-lbl:PartPackaging;
      rdfs:range xsd:string ; 
      rdfs:label "BatchCounter"@en ;
      rdfs:comment "Batch Counter identifies the number of batches (1 or max. 2 batches per reel possible)."@en ;
      skos:notation "20T"^^mat-lbl:DataID ; 
.

mat-lbl:firstBatchNumber 
      a owl:DatatypeProperty ;
      rdfs:domain mat-lbl:PartPackaging;
      rdfs:range xsd:string ; 
      rdfs:label "FirstBatchNumber"@en ;
      rdfs:comment "With this number the supplier has to be able to retroactively provide information about the batch (e.g. volume, production, delivery) A batch identification should be based on same manufacturing conditions. If a manufacturing condition changes, the batch number should be changed, too."@en ;
      skos:notation "1T"^^mat-lbl:DataID ; 
.

mat-lbl:secondBatchNumber 
      a owl:DatatypeProperty ;
      rdfs:domain mat-lbl:PartPackaging;
      rdfs:range xsd:string ; 
      rdfs:label "SecondBatchNumber"@en ;
      rdfs:comment "Batch number for the second batch - if applicable."@en ;
      skos:notation "2T"^^mat-lbl:DataID ; 
.

mat-lbl:supplierData 
      a owl:DatatypeProperty ;
      rdfs:domain mat-lbl:PartPackaging;
      rdfs:range xsd:string ; 
      rdfs:label "SupplierData"@en ;
      rdfs:comment "Supplier own information that may be used by the supplier."@en ;
      skos:notation "1Z"^^mat-lbl:DataID ; 
.

################ Printed label

mat-lbl:PrintedEntry 
      rdf:type owl:Class ;
      rdfs:label "PrintedEntry"@en ;
      rdfs:comment "..."@en ;
.

mat-lbl:hasExactLength
      rdf:type owl:DatatypeProperty ;
      rdfs:label "hasExactLength"@en ;
      rdfs:comment "..."@en ;
      rdfs:domain mat-lbl:PrintedEntry ;
      rdfs:range xsd:int ;
.

mat-lbl:hasMaximalLength
      rdf:type owl:DatatypeProperty ;
      rdfs:label "hasMaximalLength"@en ;
      rdfs:comment "..."@en ;
      rdfs:domain mat-lbl:PrintedEntry ;
      rdfs:range xsd:int ;
.

# A string for a description.
mat-lbl:hasFormat
      rdf:type owl:DatatypeProperty ;
      rdfs:label "hasFormat"@en ;
      rdfs:comment "..."@en ;
      rdfs:domain mat-lbl:PrintedEntry ;
      rdfs:range xsd:string ;
.

################ Physical aspects

mat-lbl:PhysicalLabel
      rdf:type owl:Class ;
      rdfs:label "PhysicalLabel"@en ;
      rdfs:comment "Recycling regulations have to be obeyed."@en ;
.

mat-lbl:hasPhysicalLabel
      rdf:type owl:ObjectProperty ;
      rdfs:label "hasPhysicalLabel"@en ;
      rdfs:comment "The set of data fields printed on the physical label."@en ;
      rdfs:domain mat-lbl:MatLabel ;
      rdfs:range mat-lbl:PhysicalLabel ;
.

mat-lbl:hasPrintedEntry
      rdf:type owl:ObjectProperty ;
      rdfs:label "hasPrintedEntry"@en ;
      rdfs:comment "Not all data fields have to be printed if the label is small."@en ;
      rdfs:domain mat-lbl:PhysicalLabel ;
      rdfs:range mat-lbl:PrintedEntry ;
.

# A string for a description.
mat-lbl:hasSize
      rdf:type owl:DatatypeProperty ;
      rdfs:label "hasSize"@en ;
      rdfs:comment "The size of the MAT-Label can be chosen by the supplier considering the size of the smallest package unit."@en ;
      rdfs:domain mat-lbl:PhysicalLabel ;
      rdfs:range xsd:string ;  
.

# A string for a description.
mat-lbl:hasLayout
      rdf:type owl:DatatypeProperty ;
      rdfs:label "hasLayout"@en ;
      rdfs:comment "To ensure to have enough free space for the code, its quiet zone and for the plain text, create a layout with maximum filled data fields."@en ;
      rdfs:domain mat-lbl:PhysicalLabel ;
      rdfs:range xsd:string ;  
.

mat-lbl:Adhesive
      rdf:type owl:Class ;
      rdfs:label "Adhesive"@en ;
      rdfs:comment "Material for the back of physical labels."@en ;
      owl:oneOf (mat-lbl:permanent mat-lbl:removable) ;
.

mat-lbl:permanent rdf:type owl:NamedIndividual ; 
      rdfs:label "permanent"@en ;
      rdfs:comment "Long lasting material used for the back of physical labels."@en ;
.

mat-lbl:removable rdf:type owl:NamedIndividual ; 
     rdfs:label "removable"@en ;
     rdfs:comment "Residue-free material used for the back of physical labels."@en ;
.

mat-lbl:hasAdhesive
      rdf:type owl:ObjectProperty ;
      rdfs:label "hasAdhesive"@en ;
      rdfs:comment "Applies to physical labels."@en ;
      rdfs:domain mat-lbl:PhysicalLabel ;
      rdfs:range mat-lbl:Adhesive ; 
.

# This class is characterized by having a permanent adhesive.
mat-lbl:NonremovableLabel
      rdf:type owl:Class ;
      rdfs:subClassOf mat-lbl:PhysicalLabel ;
      rdfs:subClassOf [ rdf:type owl:Restriction ;
           owl:onProperty mat-lbl:hasAdhesive ;
           owl:hasValue mat-lbl:permanent
           ] ;
      rdfs:label "NonremovableLabel"@en ;
      rdfs:comment "With permanent adhesive adjusted to the material of the smallest package unit."@en ;
.

# This class is characterized by having a removable adhesive.
mat-lbl:PeelableLabel
      rdf:type owl:Class ;
      rdfs:subClassOf mat-lbl:PhysicalLabel ;
      rdfs:subClassOf [ rdf:type owl:Restriction ;
           owl:onProperty mat-lbl:hasAdhesive ;
           owl:hasValue mat-lbl:removable
           ] ;
      rdfs:label "PeelableLabel"@en ;
      rdfs:comment "With removable adhesive adjusted to the material of the smallest package unit, residue free."@en ;
.

_:x rdf:type owl:AllDisjointClasses ;
      owl:members ( mat-lbl:NonremovableLabel mat-lbl:PeelableLabel ) .

mat-lbl:FaceMaterial
      rdf:type owl:Class ;
      rdfs:label "FaceMaterial"@en ;
      rdfs:comment "Applies to physical labels."@en ;
      owl:oneOf (mat-lbl:white mat-lbl:reversecoated mat-lbl:mat) ;
.

mat-lbl:white rdf:type owl:NamedIndividual ; 
      rdfs:label "white"@en ;
      rdfs:comment "White material used for the front of physical labels."@en ;
.

mat-lbl:reversecoated rdf:type owl:NamedIndividual ; 
      rdfs:label "reversecoated"@en ;
      rdfs:comment "Reverse coated material used for the front of physical labels."@en ;
.

mat-lbl:mat rdf:type owl:NamedIndividual ; 
      rdfs:label "mat"@en ;
      rdfs:comment "Mat material used for the front of physical labels."@en ;
.

mat-lbl:hasFaceMaterial
      rdf:type owl:ObjectProperty ;
      rdfs:label "hasFaceMaterial"@en ;
      rdfs:comment "Material for the face of physical labels."@en ;
      rdfs:domain mat-lbl:PhysicalLabel ;
      rdfs:range mat-lbl:FaceMaterial ; 
.

################ Instances

mat-lbl:matLabelA rdf:type mat-lbl:MatLabel ;
      mat-lbl:hasDataField mat-lbl:a12s ;
      mat-lbl:hasDataField mat-lbl:ap ;
      mat-lbl:hasDataField mat-lbl:a1p ;
      mat-lbl:hasDataField mat-lbl:a31p ;
      mat-lbl:hasDataField mat-lbl:a12v ;
      mat-lbl:hasDataField mat-lbl:a10v ;
      mat-lbl:hasDataField mat-lbl:a2p ;
      mat-lbl:hasDataField mat-lbl:a20p ;
      mat-lbl:hasDataField mat-lbl:a6d ;
      mat-lbl:hasDataField mat-lbl:a14d ;
      mat-lbl:hasDataField mat-lbl:a30p ;
      mat-lbl:hasDataField mat-lbl:az ;
      mat-lbl:hasDataField mat-lbl:ak ;
      mat-lbl:hasDataField mat-lbl:a16k ;
      mat-lbl:hasDataField mat-lbl:av ;
      mat-lbl:hasDataField mat-lbl:a3s ;
      mat-lbl:hasDataField mat-lbl:aq ;
      mat-lbl:hasDataField mat-lbl:a20t ;
      mat-lbl:hasDataField mat-lbl:a1t ;
      mat-lbl:hasDataField mat-lbl:a2t ;
      mat-lbl:hasDataField mat-lbl:a1z ;
.

mat-lbl:a12s rdf:type mat-lbl:DataField ;
      mat-lbl:hasDataContent "0002" ;
.

mat-lbl:ap rdf:type mat-lbl:DataField ;
      mat-lbl:hasDataContent "718.187-04 A2C5321641900" ;
.

mat-lbl:a1p rdf:type mat-lbl:DataField ;
      mat-lbl:hasDataContent "SL105C103MAA-S" ;
.

mat-lbl:a31p rdf:type mat-lbl:DataField ;
      mat-lbl:hasDataContent "SC441427CFNR2 A2C53216419/02" ;
.

mat-lbl:a12v rdf:type mat-lbl:DataField ;
      mat-lbl:hasDataContent "123456789" ;
.

mat-lbl:a10v rdf:type mat-lbl:DataField ;
      mat-lbl:hasDataContent "DEU-BERLIN CHN-BEIJING" ;
.

mat-lbl:a2p rdf:type mat-lbl:DataField ;
      mat-lbl:hasDataContent "AA 01" ;
.

mat-lbl:a20p rdf:type mat-lbl:DataField ;
      mat-lbl:hasDataContent "20 lumens" ;
.

mat-lbl:a6d rdf:type mat-lbl:DataField ;
      mat-lbl:hasDataContent "20080330" ;
.

mat-lbl:a14d rdf:type mat-lbl:DataField ;
      mat-lbl:hasDataContent "20081031" ;
.

mat-lbl:a30p rdf:type mat-lbl:DataField ;
      mat-lbl:hasDataContent "Y" ;
.

mat-lbl:az rdf:type mat-lbl:DataField ;
      mat-lbl:hasDataContent "5" ;
.

mat-lbl:ak rdf:type mat-lbl:DataField ;
      mat-lbl:hasDataContent "753013" ;
.

mat-lbl:a16k rdf:type mat-lbl:DataField ;
      mat-lbl:hasDataContent "54003333" ;
.

mat-lbl:av rdf:type mat-lbl:DataField ;
      mat-lbl:hasDataContent "884566" ;
.

mat-lbl:a3s rdf:type mat-lbl:DataField ;
      mat-lbl:hasDataContent "S123456789012" ;
.

mat-lbl:aq rdf:type mat-lbl:DataField ;
      mat-lbl:hasDataContent "1000NAR000" ;
.

mat-lbl:a20t rdf:type mat-lbl:DataField ;
      mat-lbl:hasDataContent "2" ;
.

mat-lbl:a1t rdf:type mat-lbl:DataField ;
      mat-lbl:hasDataContent "750160429" ;
.

mat-lbl:a2t rdf:type mat-lbl:DataField ;
      mat-lbl:hasDataContent "750160430" ;
.

mat-lbl:a1z rdf:type mat-lbl:DataField ;
      mat-lbl:hasDataContent "Special delivery" ;
.


# TEST DATA

conti:Automotive_Hungary a dbo:Company ;
	rdfs:label "Continental Automotive Hungary"@de ;
. 

conti:Sample_Corporation a dbo:Company ;
	rdfs:label "Sample & Co."@de ;
. 


conti:sensor123 a mat-lbl:PartPackaging ;
				mat-lbl:customerPartNumber "A2C0005836000" ;
				mat-lbl:manufacturerPartNumber "52ZIO5-31..78" ; 
				mat-lbl:orderingCode "52ZIO5-31..78" ;
				mat-lbl:partDescription "Pressure Sensor" ; 
				mat-lbl:manufacturerLocation "MEX-TORREON" ;
				mat-lbl:expirationDate "20150306" ; 
				mat-lbl:msLevel "N" ;
				mat-lbl:shippingNoteNumber "2014-53006" ; 
				mat-lbl:packageId "S4065212024201" ;
				mat-lbl:quantity 400 ;
				mat-lbl:firstBatchNumber "5300621" ;
				mat-lbl:supplierId "354325" ;
				mat-lbl:supplierData "Warehouse 4, Gate 16A" ;
				mat-lbl:supplierName "Sample & Co." ;
				mat-lbl:hasSupplier conti:Sample_Corporation ;
				mat-lbl:hasCustomer conti:Automotive_Hungary ; 
				.